Relations.v
@@ -1,0 +1,235 @@
+Require Import
+  Coq.Relations.Relation_Definitions
+  Coq.Relations.Relation_Operators
+  Coq.Relations.Operators_Properties.
+
+Require Import
+  Coq.Program.Basics
+  Coq.Classes.RelationClasses
+  Coq.Classes.Morphisms.
+
+Require Import
+  Setoid.
+
+#[global]
+Add Parametric Relation : Prop impl
+  reflexivity proved by impl_Reflexive
+  transitivity proved by impl_Transitive
+  as PreOrder_impl.
+
+Section Classes.
+  Context
+    {A : Type}
+    (R : relation A).
+
+  Class Connex :
+    Prop :=
+    connexity :
+    forall
+    x y : A,
+    R x y \/
+    R y x.
+
+  Class Functional :
+    Prop :=
+    functionality :
+    forall
+    x y y' : A,
+    R x y ->
+    R x y' ->
+    y = y'.
+
+  #[global]
+  Instance Asymmetric_Irreflexive (Asymmetric_R : Asymmetric R) : Irreflexive R.
+  Proof.
+    intros x R_x_x.
+    now apply asymmetry with x x.
+  Qed.
+End Classes.
+
+Section Restriction.
+  Context
+    {A : Type}
+    (P : A -> Prop)
+    (R : relation A).
+
+  Definition Restriction :
+    relation (sig P) :=
+    fun x y => R (proj1_sig x) (proj1_sig y).
+
+  Let R' :
+    relation (sig P) :=
+    Restriction.
+
+  #[global]
+  Instance reflexive {Reflexive_R : Reflexive R} :
+    Reflexive R'.
+  Proof.
+    intros (x & P_x).
+    apply Reflexive_R.
+  Qed.
+
+  #[global]
+  Instance irreflexive {Irreflexive_R : Irreflexive R} :
+    Irreflexive R'.
+  Proof.
+    intros (x & P_x).
+    apply Irreflexive_R.
+  Qed.
+
+  #[global]
+  Instance symmetric {Symmetric_R : Symmetric R} :
+    Symmetric R'.
+  Proof.
+    intros (x & P_x) (y & P_y).
+    apply Symmetric_R.
+  Qed.
+
+  #[global]
+  Instance asymmetric {Asymmetric_R : Asymmetric R} :
+    Asymmetric R'.
+  Proof.
+    intros (x & P_x) (y & P_y).
+    apply Asymmetric_R.
+  Qed.
+
+  #[global]
+  Instance transitive {Transitive_R : Transitive R} :
+    Transitive R'.
+  Proof.
+    intros (x & P_x) (y & P_y) (z & P_z).
+    apply Transitive_R.
+  Qed.
+
+  #[global]
+  Instance preorder {PreOrder_R : PreOrder R} :
+    PreOrder R'.
+  Proof.
+    constructor; eauto with typeclass_instances.
+  Qed.
+
+  #[global]
+  Instance equivalence {Equivalence_R : Equivalence R} :
+    Equivalence R'.
+  Proof.
+    constructor; eauto with typeclass_instances.
+  Qed.
+End Restriction.
+
+Section PartialOrder.
+  Context
+    {A : Type}
+    (P : A -> Prop)
+    (R Eq : relation A).
+
+  Let R' :
+    relation (sig P) :=
+    Restriction P R.
+
+  Let Eq' :
+    relation (sig P) :=
+    Restriction P Eq.
+
+  #[global]
+  Instance antisymmetric `{Antisymmetric_R : Antisymmetric A R Eq} :
+    Antisymmetric (sig P) R' Eq'.
+  Proof.
+    intros (x & P_x) (y & P_y).
+    apply Antisymmetric_R.
+  Qed.
+
+  #[global]
+  Instance partial_order `{PartialOrder_R : PartialOrder A R Eq} :
+    PartialOrder R' Eq'.
+  Proof.
+    intros (x & P_x) (y & P_y).
+    apply PartialOrder_R.
+  Qed.
+End PartialOrder.
+
+Module ReflexiveTransitive.
+  Section ReflexiveTransitive.
+    Context
+      {A : Type}
+      (R : relation A).
+
+    Definition Closure :
+      relation A :=
+      clos_refl_trans_1n _ R.
+
+    #[global]
+    Instance subrelation :
+      subrelation R Closure.
+    Proof.
+      intros x y R_x_y.
+      now apply clos_rt1n_step.
+    Qed.
+
+    #[global]
+    Instance reflexive :
+      Reflexive Closure.
+    Proof.
+      intros x.
+      apply rt1n_refl.
+    Qed.
+
+    #[global]
+    Instance transitive :
+      Transitive Closure.
+    Proof.
+      intros x y z; unfold Closure.
+      rewrite <- 3!clos_rt_rt1n_iff.
+      now constructor 3 with y.
+    Qed.
+
+    #[global]
+    Add Parametric Relation : A Closure
+      reflexivity proved by reflexive
+      transitivity proved by transitive
+      as preorder.
+
+    Add Parametric Morphism
+      {B : Type}
+      (S : relation B)
+      (f : A -> B)
+      `{PreOrder_R : PreOrder B S}
+      `{Proper_f : Proper (A -> B) (R ++> S)%signature f} : f with signature
+      Closure ++> S as morphism.
+    Proof.
+      intros x y Closure_x_y.
+      induction Closure_x_y as
+        [x|
+      x x' y R_x_x' Closure_x'_y IHx'_y].
+        reflexivity.
+      now transitivity (f x'); [rewrite R_x_x'|].
+    Qed.
+  End ReflexiveTransitive.
+
+  Section Restriction.
+    Variables
+      (A : Type)
+      (P : A -> Prop)
+      (R : relation A)
+      (Proper_P : Proper (R ++> impl) P)
+      (x y : A)
+      (P_x : P x).
+
+    Lemma Restriction :
+      Closure R x y ->
+      exists
+      P_y : P y,
+      Closure
+        (Restriction P R)
+        (exist P x P_x)
+        (exist P y P_y).
+    Proof.
+      induction 1 as
+        [x|
+      x x' y R_x_x' Closure_x'_y IHx'_y].
+        now exists P_x.
+      assert (P_x' : P x') by now rewrite <- R_x_x'.
+      specialize IHx'_y with P_x' as (P_y & H).
+      now exists P_y; constructor 2 with (exist P x' P_x').
+    Qed.
+  End Restriction.
+End ReflexiveTransitive.
